# Zeros of a Polynomial Using Zero Product Property

## Given Function
We are given the polynomial function:

h(x) = (-4x - 3)(x - 3)

---

## Objective
To find the **zeros of the polynomial** using the  
**Zero Product Property**.

---

## Zero Product Property
The **Zero Product Property** states that:

> If the product of two or more factors is zero,  
> then at least one of the factors must be zero.

Mathematically:
If  
(a)(b) = 0  
then  
a = 0 or b = 0

---

## Applying the Property

Given:
(-4x - 3)(x - 3) = 0

Set each factor equal to zero.

---

### Step 1
-4x - 3 = 0  

-4x = 3  

x = -3/4

---

### Step 2
x - 3 = 0  

x = 3

---

## Final Answer
The zeros of the polynomial are:

**x = -3/4 and x = 3**

---

## Conclusion
By applying the Zero Product Property, we were able to find
the zeros of the polynomial easily.

This method is:
- clear,
- exam-friendly, and
- useful when the polynomial is already factorised.
